theories/tree_borrows/disjoint.v
@@ -6,15 +6,15 @@ From iris.prelude Require Import options.
 (* Key lemma: converts the entire traversal to a per-node level.
    This is applicable to every permission in the accessed range, all that's needed
    to complement it should be preservation of permissions outside of said range. *)
-Lemma access_effect_per_loc_within_range tr affected_tag access_tag pre :
-  tree_contains access_tag tr ->
-  tree_contains affected_tag tr ->
-  tree_unique affected_tag pre tr ->
-  forall kind strong cids range tr' z zpre,
-  range_contains range z ->
-  item_lazy_perm_at_loc pre z = zpre ->
-  tree_apply_access (item_apply_access kind strong) cids access_tag range tr (naive_rel_dec tr) = Some tr' ->
-  exists post zpost, (
+Lemma access_effect_per_loc_within_range
+  tr affected_tag access_tag pre
+  (Ex : tree_contains affected_tag tr)
+  (Unq : tree_unique affected_tag pre tr)
+  kind strong cids cids' range tr' z zpre
+  (Within : range_contains range z)
+  (IsPre : item_lazy_perm_at_loc pre z = zpre)
+  (Step : bor_local_step tr cids (AccessBLEvt kind strong access_tag range) tr' cids')
+  : exists post zpost, (
     let rel := if naive_rel_dec tr affected_tag access_tag then AccessChild else AccessForeign in
     let isprot := bool_decide (protector_is_active cids pre.(iprot)) in
     let isstrong := bool_decide (strong = ProtStrong \/ protector_is_strong pre.(iprot)) in
@@ -24,21 +24,20 @@ Lemma access_effect_per_loc_within_range tr affected_tag access_tag pre :
     /\ iprot post = iprot pre
   ).
 Proof.
-  intros ContainsAcc ContainsAff UniqueAff kind strong cids range tr' z zpre WithinRange IsPre Success.
+  inversion Step; subst.
   (* use apply_access_spec_per_node to get info on the post permission *)
   destruct (apply_access_spec_per_node _ _ _ _
-    ContainsAcc ContainsAff UniqueAff
-    (item_apply_access _ _) cids range tr' (naive_rel_dec tr)
-    (item_apply_access_preserves_tag _ _) Success) as [post [SpecPost [ContainsPost UniquePost]]].
-  clear Success.
+    EXISTS_TAG Ex Unq
+    (item_apply_access _ _) cids' range tr' (naive_rel_dec tr)
+    (item_apply_access_preserves_tag _ _) ACC) as [post [SpecPost [ContainsPost UniquePost]]].
   (* and then it's per-tag work *)
-  rewrite (tree_unique_specifies_tag _ _ _ ContainsAff UniqueAff) in SpecPost.
+  rewrite (tree_unique_specifies_tag _ _ _ Ex Unq) in SpecPost.
   symmetry in SpecPost.
   destruct (option_bind_success_step _ _ _  SpecPost) as [tmpperm [tmpSpec tmpRes]].
   injection tmpRes; intro H; subst; clear tmpRes.
   (* now down to per-location *)
   pose proof (range_foreach_spec _ _ z _ _ tmpSpec) as ForeachSpec.
-  rewrite (decide_True _ _ WithinRange) in ForeachSpec.
+  rewrite (decide_True _ _ Within) in ForeachSpec.
   destruct ForeachSpec as [lazy_perm [PermExists ForeachSpec]].
   assert (unwrap {| initialized := PermLazy; perm := initp pre |} (iperm pre !! z) = item_lazy_perm_at_loc pre z) as InitPerm. {
     unfold item_lazy_perm_at_loc. destruct (iperm pre !! z); simpl; reflexivity.
@@ -49,26 +48,27 @@ Proof.
   unfold item_lazy_perm_at_loc.
   rewrite PermExists; simpl; reflexivity.
 Qed.
+Arguments access_effect_per_loc_within_range {_ _ _ _} Ex Unq {_ _ _ _ _ _ _ _} Within IsPre Step.
 
-Lemma access_effect_per_loc_outside_range tr affected_tag access_tag pre :
-  tree_contains access_tag tr ->
-  tree_contains affected_tag tr ->
-  tree_unique affected_tag pre tr ->
-  forall kind strong cids range tr' z zpre,
-  ~range_contains range z ->
-  item_lazy_perm_at_loc pre z = zpre ->
-  tree_apply_access (item_apply_access kind strong) cids access_tag range tr (naive_rel_dec tr) = Some tr' ->
-  exists post, (
+Lemma access_effect_per_loc_outside_range
+  tr affected_tag access_tag pre
+  (Ex : tree_contains affected_tag tr)
+  (Unq : tree_unique affected_tag pre tr)
+  kind strong cids cids' range tr' z zpre
+  (Outside : ~range_contains range z)
+  (IsPre : item_lazy_perm_at_loc pre z = zpre)
+  (Step : bor_local_step tr cids (AccessBLEvt kind strong access_tag range) tr' cids')
+  : exists post, (
     tree_unique affected_tag post tr
     /\ item_lazy_perm_at_loc post z = zpre
     /\ iprot post = iprot pre
   ).
 Proof.
-  intros ContainsAcc ContainsAff UniqueAff kind strong cids range tr' z zpre OutsideRange IsPre Success.
+  inversion Step; subst.
   destruct (apply_access_spec_per_node _ _ _ _
-    ContainsAcc ContainsAff UniqueAff _ _ _ _ _
+    EXISTS_TAG Ex Unq _ _ _ _ _
     (item_apply_access_preserves_tag _ _)
-    Success) as [post [SpecPost [ContainsPost UniquePost]]].
+    ACC) as [post [SpecPost [ContainsPost UniquePost]]].
   (* We now show that
      (1) post has zpre at loc z
      (2) post is equal to whatever item the goal refers to *)
@@ -77,35 +77,34 @@ Proof.
     destruct (option_bind_success_step _ _ _ SpecPost) as [perms [SpecPerms Injectable]].
     injection Injectable; intros; subst; clear Injectable.
     pose proof (range_foreach_spec _ _ z _ _ SpecPerms) as RangeForeach.
-    rewrite (decide_False _ _ OutsideRange) in RangeForeach.
+    rewrite (decide_False _ _ Outside) in RangeForeach.
     unfold item_lazy_perm_at_loc; simpl.
     rewrite RangeForeach; reflexivity.
   }
   eexists.
-  split; [|split]; [exact UniqueAff|apply IsPre|reflexivity].
+  split; [|split]; [exact Unq|reflexivity|reflexivity].
 Qed.
+Arguments access_effect_per_loc_outside_range {_ _ _ _} Ex Unq {_ _ _ _ _ _ _ _} Outside IsPre Step.
 
-Lemma nonchild_write_reserved_to_disabled tr affected_tag access_tag pre :
-  tree_contains access_tag tr ->
-  tree_contains affected_tag tr ->
-  tree_unique affected_tag pre tr ->
-  ~ParentChildIn affected_tag access_tag tr ->
-  forall cids range tr' z zpre,
-  range_contains range z ->
-  item_lazy_perm_at_loc pre z = zpre ->
-  reach Reserved (perm zpre) ->
-  memory_access AccessWrite ProtStrong cids access_tag range tr = Some tr' ->
-  exists post zpost, (
+Lemma nonchild_write_reserved_to_disabled
+  {tr affected_tag access_tag pre}
+  (Ex : tree_contains affected_tag tr)
+  (Unq : tree_unique affected_tag pre tr)
+  (Nonchild : ~ParentChildIn affected_tag access_tag tr)
+  {cids cids' range tr' z zpre}
+  (Within : range_contains range z)
+  (IsPre : item_lazy_perm_at_loc pre z = zpre)
+  (Reach : reach Reserved (perm zpre))
+  (Step : bor_local_step tr cids (AccessBLEvt AccessWrite ProtStrong access_tag range) tr' cids')
+  : exists post zpost, (
     tree_unique affected_tag post tr'
     /\ item_lazy_perm_at_loc post z = zpost
     /\ reach Disabled (perm zpost)
     /\ iprot post = iprot pre
   ).
 Proof.
-  intros ContainsAcc ContainsAff UniqueAff Nonrel cids range tr' z zpre WithinRange preLoc NonResMut Write.
-  destruct (access_effect_per_loc_within_range _ _ _ _
-    ContainsAcc ContainsAff UniqueAff
-    AccessWrite ProtStrong cids range tr' z zpre WithinRange preLoc Write) as [post [zpost [SpecPost [UniqPost [PermPost ProtPost]]]]].
+  destruct (access_effect_per_loc_within_range Ex Unq Within IsPre Step)
+    as [post [zpost [SpecPost [UniqPost [PermPost ProtPost]]]]].
   exists post, zpost.
   try repeat split; auto.
   destruct (naive_rel_dec _ _ _); [contradiction|].
@@ -115,27 +114,25 @@ Proof.
   all: simpl; tauto.
 Qed.
 
-Lemma nonchild_read_active_to_frozen tr affected_tag access_tag pre :
-  tree_contains access_tag tr ->
-  tree_contains affected_tag tr ->
-  tree_unique affected_tag pre tr ->
-  ~ParentChildIn affected_tag access_tag tr ->
-  forall cids range tr' z zpre,
-  range_contains range z ->
-  item_lazy_perm_at_loc pre z = zpre ->
-  reach Active (perm zpre) ->
-  memory_access AccessRead ProtStrong cids access_tag range tr = Some tr' ->
-  exists post zpost, (
+Lemma nonchild_read_active_to_frozen
+  {tr affected_tag access_tag pre}
+  (Ex : tree_contains affected_tag tr)
+  (Unq : tree_unique affected_tag pre tr)
+  (Nonchild : ~ParentChildIn affected_tag access_tag tr)
+  {cids cids' range tr' z zpre}
+  (Within : range_contains range z)
+  (IsPre : item_lazy_perm_at_loc pre z = zpre)
+  (Reach : reach Active (perm zpre))
+  (Step : bor_local_step tr cids (AccessBLEvt AccessRead ProtStrong access_tag range) tr' cids')
+  : exists post zpost, (
     tree_unique affected_tag post tr'
     /\ item_lazy_perm_at_loc post z = zpost
     /\ reach Frozen (perm zpost)
     /\ reach (perm zpre) (perm zpost)
   ).
 Proof.
-  intros ContainsAcc ContainsAff UniqueAff Nonrel cids range tr' z zpre WithinRange preLoc NonResMut Read.
-  destruct (access_effect_per_loc_within_range _ _ _ _
-    ContainsAcc ContainsAff UniqueAff
-    AccessRead ProtStrong cids range tr' z zpre WithinRange preLoc Read) as [post [zpost [SpecPost [UniqPost [PermPost ProtPost]]]]].
+  destruct (access_effect_per_loc_within_range Ex Unq Within IsPre Step)
+    as [post [zpost [SpecPost [UniqPost [PermPost ProtPost]]]]].
   exists post, zpost.
   try repeat split; auto.
   all: destruct (naive_rel_dec _ _ _); [contradiction|].
@@ -145,59 +142,56 @@ Proof.
   all: simpl; tauto.
 Qed.
 
-Lemma child_write_frozen_to_ub tr affected_tag access_tag pre :
-  tree_contains access_tag tr ->
-  tree_contains affected_tag tr ->
-  tree_unique affected_tag pre tr ->
-  ParentChildIn affected_tag access_tag tr ->
-  forall cids range tr' z zpre,
-  range_contains range z ->
-  item_lazy_perm_at_loc pre z = zpre ->
-  reach Frozen (perm zpre) ->
-  memory_access AccessWrite ProtStrong cids access_tag range tr = Some tr' ->
-  False.
+Lemma child_write_frozen_to_ub
+  {tr affected_tag access_tag pre}
+  (Ex : tree_contains affected_tag tr)
+  (Unq : tree_unique affected_tag pre tr)
+  (Child : ParentChildIn affected_tag access_tag tr)
+  {cids cids' range tr' z zpre}
+  (Within : range_contains range z)
+  (IsPre : item_lazy_perm_at_loc pre z = zpre)
+  (Reach : reach Frozen (perm zpre))
+  (Step : bor_local_step tr cids (AccessBLEvt AccessWrite ProtStrong access_tag range) tr' cids')
+  : False.
 Proof.
-  intros ContainsAcc ContainsAff UniqueAff Related cids range tr' z zpre WithinRange PermPre ReachFrz Write.
-  destruct (access_effect_per_loc_within_range _ _ _ _
-  ContainsAcc ContainsAff UniqueAff
-  AccessWrite ProtStrong cids range tr' z zpre WithinRange PermPre Write) as [post [zpost [SpecPost [UniqPost [PermPost ProtPost]]]]].
+  destruct (access_effect_per_loc_within_range Ex Unq Within IsPre Step)
+    as [post [zpost [SpecPost [UniqPost [PermPost ProtPost]]]]].
   destruct (naive_rel_dec _ _ _); [|contradiction].
   destruct zpre; destruct initialized; destruct perm; try contradiction.
   all: destruct (bool_decide _); simpl in *.
   all: try inversion SpecPost.
 Qed.
 
-Lemma child_read_disabled_to_ub tr affected_tag access_tag pre :
-  tree_contains access_tag tr ->
-  tree_contains affected_tag tr ->
-  tree_unique affected_tag pre tr ->
-  ParentChildIn affected_tag access_tag tr ->
-  forall cids range tr' z zpre,
-  range_contains range z ->
-  item_lazy_perm_at_loc pre z = zpre ->
-  reach Disabled (perm zpre) ->
-  memory_access AccessRead ProtStrong cids access_tag range tr = Some tr' ->
-  False.
+Lemma child_read_disabled_to_ub
+  {tr affected_tag access_tag pre}
+  (Ex : tree_contains affected_tag tr)
+  (Unq : tree_unique affected_tag pre tr)
+  (Child : ParentChildIn affected_tag access_tag tr)
+  {cids cids' range tr' z zpre}
+  (Within : range_contains range z)
+  (IsPre : item_lazy_perm_at_loc pre z = zpre)
+  (Reach : reach Disabled (perm zpre))
+  (Step : bor_local_step tr cids (AccessBLEvt AccessRead ProtStrong access_tag range) tr' cids')
+  : False.
 Proof.
-  intros ContainsAcc ContainsAff UniqueAff Related cids range tr' z zpre WithinRange PermPre ReachFrz Read.
-  destruct (access_effect_per_loc_within_range _ _ _ _
-    ContainsAcc ContainsAff UniqueAff
-    AccessRead ProtStrong cids range tr' z zpre WithinRange PermPre Read) as [post [zpost [SpecPost [UniqPost [PermPost ProtPost]]]]].
+  destruct (access_effect_per_loc_within_range Ex Unq Within IsPre Step)
+    as [post [zpost [SpecPost [UniqPost [PermPost ProtPost]]]]].
   destruct (naive_rel_dec _ _ _); [|contradiction].
   destruct zpre; destruct initialized; destruct perm; try contradiction.
   all: destruct (bool_decide _); simpl in *.
   all: try inversion SpecPost.
 Qed.
 
-Lemma child_write_any_to_init_active tr affected_tag access_tag pre :
-  tree_contains access_tag tr ->
-  tree_contains affected_tag tr ->
-  tree_unique affected_tag pre tr ->
-  ParentChildIn affected_tag access_tag tr ->
-  forall cids range tr' z,
-  range_contains range z ->
-  memory_access AccessWrite ProtStrong cids access_tag range tr = Some tr' ->
-  exists post zpost, (
+Lemma child_write_any_to_init_active
+  {tr affected_tag access_tag pre}
+  (Ex : tree_contains affected_tag tr)
+  (Unq : tree_unique affected_tag pre tr)
+  (Child : ParentChildIn affected_tag access_tag tr)
+  {cids cids' range tr' z zpre}
+  (Within : range_contains range z)
+  (IsPre : item_lazy_perm_at_loc pre z = zpre)
+  (Step : bor_local_step tr cids (AccessBLEvt AccessWrite ProtStrong access_tag range) tr' cids')
+  : exists post zpost, (
     tree_unique affected_tag post tr'
     /\ item_lazy_perm_at_loc post z = zpost
     /\ perm zpost = Active
@@ -205,30 +199,30 @@ Lemma child_write_any_to_init_active tr affected_tag access_tag pre :
     /\ initialized zpost = PermInit
   ).
 Proof.
-  intros ContainsAcc ContainsAff UniqueAff Related cids range tr' z WithinRange Write.
-  destruct (access_effect_per_loc_within_range _ _ _ _
-    ContainsAcc ContainsAff UniqueAff
-    AccessWrite ProtStrong cids range tr' z
-    (item_lazy_perm_at_loc pre z) WithinRange ltac:(reflexivity) Write) as [post [zpost [SpecPost [UniqPost [PermPost ProtPost]]]]].
+  destruct (access_effect_per_loc_within_range Ex Unq Within IsPre Step)
+    as [post [zpost [SpecPost [UniqPost [PermPost ProtPost]]]]].
   destruct (naive_rel_dec _ _ _); [|contradiction].
   exists post, zpost.
   try repeat split; try assumption.
   all: destruct (item_lazy_perm_at_loc _ _); destruct initialized; destruct perm; try contradiction.
   all: destruct (bool_decide _); simpl in *.
   all: unfold apply_access_perm in SpecPost; simpl in *.
+  all: destruct (perm zpre); simpl in *.
+  all: destruct (initialized zpre); simpl in *.
   all: try inversion SpecPost.
   all: injection SpecPost; intro H; destruct zpost; injection H; intros; subst; simpl; reflexivity.
 Qed.
 
-Lemma child_read_any_to_init_nondis tr affected_tag access_tag pre :
-  tree_contains access_tag tr ->
-  tree_contains affected_tag tr ->
-  tree_unique affected_tag pre tr ->
-  ParentChildIn affected_tag access_tag tr ->
-  forall cids range tr' z,
-  range_contains range z ->
-  memory_access AccessRead ProtStrong cids access_tag range tr = Some tr' ->
-  exists post zpost, (
+Lemma child_read_any_to_init_nondis
+  {tr affected_tag access_tag pre}
+  (Ex : tree_contains affected_tag tr)
+  (Unq : tree_unique affected_tag pre tr)
+  (Child : ParentChildIn affected_tag access_tag tr)
+  {cids cids' range tr' z zpre}
+  (Within : range_contains range z)
+  (IsPre : item_lazy_perm_at_loc pre z = zpre)
+  (Step : bor_local_step tr cids (AccessBLEvt AccessRead ProtStrong access_tag range) tr' cids')
+  : exists post zpost, (
     tree_unique affected_tag post tr'
     /\ item_lazy_perm_at_loc post z = zpost
     /\ ~reach Disabled (perm zpost)
@@ -236,39 +230,37 @@ Lemma child_read_any_to_init_nondis tr affected_tag access_tag pre :
     /\ initialized zpost = PermInit
   ).
 Proof.
-  intros ContainsAcc ContainsAff UniqueAff Related cids range tr' z WithinRange Read.
-  destruct (access_effect_per_loc_within_range _ _ _ _
-    ContainsAcc ContainsAff UniqueAff
-    AccessRead ProtStrong cids range tr' z
-    (item_lazy_perm_at_loc pre z) WithinRange ltac:(reflexivity) Read) as [post [zpost [SpecPost [UniqPost [PermPost ProtPost]]]]].
+  destruct (access_effect_per_loc_within_range Ex Unq Within IsPre Step)
+    as [post [zpost [SpecPost [UniqPost [PermPost ProtPost]]]]].
   destruct (naive_rel_dec _ _ _); [|contradiction].
   exists post, zpost.
   try repeat split; try assumption.
   all: destruct (item_lazy_perm_at_loc _ _); destruct initialized; destruct perm; try contradiction.
   all: destruct (bool_decide _); simpl in *.
   all: unfold apply_access_perm in SpecPost; simpl in *.
+  all: destruct (perm zpre); simpl in *.
+  all: destruct (initialized zpre); simpl in *.
   all: try inversion SpecPost.
   all: injection SpecPost; intro H; destruct zpost; simpl; tauto.
 Qed.
 
-Lemma protected_nonchild_write_initialized_to_ub tr affected_tag access_tag pre :
-  tree_contains access_tag tr ->
-  tree_contains affected_tag tr ->
-  tree_unique affected_tag pre tr ->
-  ~ParentChildIn affected_tag access_tag tr ->
-  forall cids range tr' z,
-  protector_is_active cids (iprot pre) ->
-  initialized (item_lazy_perm_at_loc pre z) = PermInit ->
-  ~reach Disabled (perm (item_lazy_perm_at_loc pre z)) ->
-  range_contains range z ->
-  memory_access AccessWrite ProtStrong cids access_tag range tr = Some tr' ->
-  False.
+
+Lemma protected_nonchild_write_initialized_to_ub
+  {tr affected_tag access_tag pre}
+  (Ex : tree_contains affected_tag tr)
+  (Unq : tree_unique affected_tag pre tr)
+  (Nonchild : ~ParentChildIn affected_tag access_tag tr)
+  {cids cids' range tr' z zpre}
+  (Protected : protector_is_active cids (iprot pre))
+  (Initialized : initialized (item_lazy_perm_at_loc pre z) = PermInit)
+  (Within : range_contains range z)
+  (IsPre : item_lazy_perm_at_loc pre z = zpre)
+  (NonDis : ~reach Disabled (perm zpre))
+  (Step : bor_local_step tr cids (AccessBLEvt AccessWrite ProtStrong access_tag range) tr' cids')
+  : False.
 Proof.
-  move=> ContainsAcc ContainsAff UniqueAff Unrelated ???? Protected Initialized NonDis WithinRange Write.
-  destruct (access_effect_per_loc_within_range _ _ _ _
-    ContainsAcc ContainsAff UniqueAff
-    AccessWrite ProtStrong _ _ _ _ _ WithinRange
-    ltac:(reflexivity) Write) as [post [zpost [SpecPost [UniquePost [PermPost ProtPost]]]]].
+  destruct (access_effect_per_loc_within_range Ex Unq Within IsPre Step)
+    as [post [zpost [SpecPost [UniqPost [PermPost ProtPost]]]]].
   destruct (naive_rel_dec _ _ _); [contradiction|].
   rewrite bool_decide_eq_true_2 in SpecPost; [|assumption].
   destruct (item_lazy_perm_at_loc _ _); simpl in Initialized; subst.
@@ -278,56 +270,52 @@ Proof.
   apply NonDis; simpl; tauto.
 Qed.
 
-Lemma protected_nonchild_read_initialized_active_to_ub tr affected_tag access_tag pre :
-  tree_contains access_tag tr ->
-  tree_contains affected_tag tr ->
-  tree_unique affected_tag pre tr ->
-  ~ParentChildIn affected_tag access_tag tr ->
-  forall cids range tr' z,
-  protector_is_active cids (iprot pre) ->
-  initialized (item_lazy_perm_at_loc pre z) = PermInit ->
-  perm (item_lazy_perm_at_loc pre z) = Active ->
-  range_contains range z ->
-  memory_access AccessRead ProtStrong cids access_tag range tr = Some tr' ->
-  False.
+Lemma protected_nonchild_read_initialized_active_to_ub
+  {tr affected_tag access_tag pre}
+  (Ex : tree_contains affected_tag tr)
+  (Unq : tree_unique affected_tag pre tr)
+  (Nonchild : ~ParentChildIn affected_tag access_tag tr)
+  {cids cids' range tr' z zpre}
+  (Protected : protector_is_active cids (iprot pre))
+  (Initialized : initialized (item_lazy_perm_at_loc pre z) = PermInit)
+  (Within : range_contains range z)
+  (IsPre : item_lazy_perm_at_loc pre z = zpre)
+  (Activated : perm zpre = Active)
+  (Step : bor_local_step tr cids (AccessBLEvt AccessRead ProtStrong access_tag range) tr' cids')
+  : False.
 Proof.
-  move=> ContainsAcc ContainsAff UniqueAff Unrelated ???? Protected Initialized Active WithinRange Read.
-  destruct (access_effect_per_loc_within_range _ _ _ _
-    ContainsAcc ContainsAff UniqueAff
-    AccessRead ProtStrong _ _ _ _ _ WithinRange
-    ltac:(reflexivity) Read) as [post [zpost [SpecPost [UniquePost [PermPost ProtPost]]]]].
+  destruct (access_effect_per_loc_within_range Ex Unq Within IsPre Step)
+    as [post [zpost [SpecPost [UniqPost [PermPost ProtPost]]]]].
   destruct (naive_rel_dec _ _ _); [contradiction|].
   rewrite bool_decide_eq_true_2 in SpecPost; [|assumption].
   destruct (item_lazy_perm_at_loc _ _); simpl in Initialized; subst.
   destruct perm; unfold apply_access_perm in SpecPost; simpl in SpecPost.
-  all: try inversion Active.
+  all: try inversion Activated.
   inversion SpecPost.
 Qed.
 
-Lemma protected_nonchild_read_any_to_frozen tr affected_tag access_tag pre :
-  tree_contains access_tag tr ->
-  tree_contains affected_tag tr ->
-  tree_unique affected_tag pre tr ->
-  ~ParentChildIn affected_tag access_tag tr ->
-  forall cids range tr' z,
-  protector_is_active cids (iprot pre) ->
-  range_contains range z ->
-  memory_access AccessRead ProtStrong cids access_tag range tr = Some tr' ->
-  exists post zpost, (
+Lemma protected_nonchild_read_any_to_frozen
+  {tr affected_tag access_tag pre}
+  (Ex : tree_contains affected_tag tr)
+  (Unq : tree_unique affected_tag pre tr)
+  (Nonchild : ~ParentChildIn affected_tag access_tag tr)
+  {cids cids' range tr' z zpre}
+  (Protected : protector_is_active cids (iprot pre))
+  (Within : range_contains range z)
+  (IsPre : item_lazy_perm_at_loc pre z = zpre)
+  (Step : bor_local_step tr cids (AccessBLEvt AccessRead ProtStrong access_tag range) tr' cids')
+  : exists post zpost, (
     tree_unique affected_tag post tr'
     /\ item_lazy_perm_at_loc post z = zpost
     /\ reach Frozen (perm zpost)
   ).
 Proof.
-  move=> ContainsAcc ContainsAff UniqueAff Unrelated ???? Protected WithinRange Read.
-  destruct (access_effect_per_loc_within_range _ _ _ _
-    ContainsAcc ContainsAff UniqueAff
-    AccessRead ProtStrong _ _ _ _ _ WithinRange
-    ltac:(reflexivity) Read) as [post [zpost [SpecPost [UniquePost [PermPost ProtPost]]]]].
+  destruct (access_effect_per_loc_within_range Ex Unq Within IsPre Step)
+    as [post [zpost [SpecPost [UniqPost [PermPost ProtPost]]]]].
   destruct (naive_rel_dec _ _ _); [contradiction|].
   rewrite bool_decide_eq_true_2 in SpecPost; [|assumption].
   eexists. eexists.
-  try repeat split; [exact UniquePost|].
+  try repeat split; [exact UniqPost|].
   destruct (item_lazy_perm_at_loc pre _); simpl in SpecPost; subst.
   destruct (item_lazy_perm_at_loc post _); simpl in SpecPost; subst.
   destruct perm; destruct initialized; simpl.
@@ -341,19 +329,19 @@ Ltac migrate prop dest :=
   (* Migrate a tree_contains *)
   | tree_contains ?tg ?tr =>
     idtac "found" tg;
-    match goal with
-    | ACC: memory_access _ _ _ _ _ ?tr = Some _ |- _ =>
-      pose proof (proj1 (access_preserves_tags _ _ _ _ _ _ _ _ (item_apply_access_preserves_tag _ _) ACC) prop) as dest
-    | ACC: create_child _ _ _ _ _ = Some _ |- _ =>
-      idtac "passing through insertion";
-      pose proof (insertion_preserves_tags _ _ _ _ _ _ _ prop ACC) as dest
+    lazymatch goal with
+    | Step: bor_local_step tr _ _ _ _ |- _ =>
+      pose proof (bor_local_step_preserves_contains prop Step) as dest
     end
   (* Migrate a parent-child relation *)
   | context [ParentChildIn ?tg ?tg' ?tr] =>
-    match goal with
-    | ACC: memory_access _ _ _ _ _ ?tr = Some _ |- _ =>
+    lazymatch goal with
+    | Step : bor_local_step tr _ _ _ _,
+      Ex : tree_contains tg tr,
+      Ex' : tree_contains tg' tr
+      |- _ =>
       pose proof prop as dest;
-      rewrite (access_eqv_rel _ _ _ _ _ _ _ _ _ (item_apply_access_preserves_tag _ _) ACC) in dest
+      rewrite (bor_local_step_eqv_rel Ex Ex' Step) in dest
     end
   (* Migrate info on a protector *)
   | context [protector_is_for_call ?old _] =>
@@ -386,11 +374,8 @@ Ltac forget x :=
 
 Ltac created_unique tg bindEx bindUnq :=
   match goal with
-  | Rebor: create_child _ ?tgp tg _ ?tr = Some _,
-    Ex: tree_contains ?tgp ?tr,
-    Fresh: ~tree_contains tg ?tr
-    |- _ =>
-      pose proof (create_child_unique _ _ _ _ Ex Fresh _ _ Rebor) as [bindEx bindUnq]
+  | Rebor : bor_local_step ?tr _ (RetagBLEvt _ tg _ _) _ _ |- _ =>
+    pose proof (bor_local_step_retag_produces_contains_unique Rebor) as [bindEx bindUnq]
   end.
 
 Tactic Notation "created" constr(tg) "unique" "as" "[" ident(ex) ident(uq) "]" :=
@@ -415,21 +400,19 @@ Tactic Notation "created" constr(tg) "protected" :=
   let prot := fresh "Protected" in
   created_protected tg prot.
 
-Ltac created_nonchild tg other dest :=
+Ltac created_nonparent tg other dest :=
   match goal with
-  | Exother : tree_contains other ?tr,
-    Exparent : tree_contains ?tgp ?tr,
-    Fresh : ~tree_contains tg ?tr,
-    Rebor : create_child _ ?tgp tg _ ?tr = Some _
+  | Rebor : bor_local_step ?tr _ (RetagBLEvt _ tg _ _) _ _,
+    Exother : tree_contains other ?tr
     |- _ =>
-    pose proof (insertion_order_nonchild _ _ _ Exother Fresh _ _ _ _ Exparent Rebor) as dest
+    pose proof (bor_local_step_retag_order_nonparent Exother Rebor) as dest
   end.
 
 Tactic Notation "created" constr(tg) "nonparent" "of" constr(other) "as" ident(dest) :=
-  created_nonchild tg other dest.
+  created_nonparent tg other dest.
 Tactic Notation "created" constr(tg) "nonparent" "of" constr(other) :=
   let unrel := fresh "Unrelated" in
-  created_nonchild tg other unrel.
+  created_nonparent tg other unrel.
 
 Ltac solve_reachability :=
   let p := fresh "perm" in
@@ -441,18 +424,42 @@ Ltac solve_reachability :=
   end.
 
 Lemma fwrite_cwrite_disjoint tg tg' newp range1 range2 :
-  forall tgp tr0 tr1 tr2 tr3 cids0 cids1 cids2,
+  forall tgp tr0 tr1 tr2 tr3 cid cids0 cids1 cids2 cids3,
   tree_contains tg tr0 ->
-  tree_contains tgp tr0 ->
-  ~tree_contains tg' tr0 ->
   reach Reserved (initial_state newp) ->
-  create_child cids0 tgp tg' newp tr0 = Some tr1 ->
-  memory_access AccessWrite ProtStrong cids1 tg range1 tr1 = Some tr2 ->
-  memory_access AccessWrite ProtStrong cids2 tg' range2 tr2 = Some tr3 ->
+  bor_local_step tr0 cids0 (RetagBLEvt tgp tg' newp cid) tr1 cids1 ->
+  bor_local_step tr1 cids1 (AccessBLEvt AccessWrite ProtStrong tg range1) tr2 cids2 ->
+  bor_local_step tr2 cids2 (AccessBLEvt AccessWrite ProtStrong tg' range2) tr3 cids3 ->
   ~exists z, range_contains range1 z /\ range_contains range2 z.
 Proof.
-  move=> ? tr0 tr1 tr2 tr3 ???.
-  intros TgEx TgpEx Tg'Fresh NonResMut Rebor Write12 Write23 [z [RContains1 RContains2]].
+  move=> ? tr0 tr1 tr2 tr3 ?????.
+  intros TgEx NonResMut Rebor Write12 Write23 [z [RContains1 RContains2]].
+  (* reborrow step *)
+  created tg' unique as [Tg'Ex Tg'Unique].
+  Check (bor_local_step_retag_order_nonparent ).
+  created tg' nonparent of tg as Unrelated.
+  forget tr0.
+
+  (* write step 1 *)
+  destruct (nonchild_write_reserved_to_disabled Tg'Ex Tg'Unique Unrelated RContains1 eq_refl ltac:(solve_reachability) Write12)
+    as [post [zpost [Unique'Post [PermPost [DisPost ProtPost]]]]].
+  migrate Tg'Ex.
+  forget tr1.
+
+  (* write step 2 *)
+  destruct (child_write_frozen_to_ub Tg'Ex Unique'Post ltac:(left; done) RContains2 PermPost ltac:(repeat solve_reachability) Write23).
+Qed.
+
+Lemma fwrite_cread_disjoint tg tg' newp range1 range2 :
+  forall tgp tr0 tr1 tr2 tr3 cid cids0 cids1 cids2 cids3,
+  tree_contains tg tr0 ->
+  reach Reserved (initial_state newp) ->
+  bor_local_step tr0 cids0 (RetagBLEvt tgp tg' newp cid) tr1 cids1 ->
+  bor_local_step tr1 cids1 (AccessBLEvt AccessWrite ProtStrong tg range1) tr2 cids2 ->
+  bor_local_step tr2 cids2 (AccessBLEvt AccessRead ProtStrong tg' range2) tr3 cids3 ->
+  ~exists z, range_contains range1 z /\ range_contains range2 z.
+Proof.
+  move=> ? tr0 tr1 tr2 tr3 ????? TgEx ReachRes Rebor Write12 Read23 [z [RContains1 RContains2]].
   (* reborrow step *)
   created tg' unique as [Tg'Ex Tg'Unique].
   created tg' nonparent of tg as Unrelated.
@@ -460,9 +467,9 @@ Proof.
   forget tr0.
 
   (* write step 1 *)
-  destruct (nonchild_write_reserved_to_disabled _ _ _ _
-    TgEx Tg'Ex Tg'Unique
-    Unrelated _ _ _ _ _
+  destruct (nonchild_write_reserved_to_disabled
+    Tg'Ex Tg'Unique
+    Unrelated
     RContains1 eq_refl
     ltac:(solve_reachability)
     Write12
@@ -470,65 +477,25 @@ Proof.
   migrate Tg'Ex.
   forget tr1.
 
-  (* write step 2 *)
-  destruct (child_write_frozen_to_ub _ _ _ _
-    Tg'Ex Tg'Ex Unique'Post
-    ltac:(left; done) _ _ _ _ _
-    RContains2 PermPost
-    ltac:(repeat solve_reachability)
-    Write23).
-Qed.
-
-Lemma fwrite_cread_disjoint tg tg' newp range1 range2 :
-  forall tgp tr0 tr1 tr2 tr3 cids0 cids1 cids2,
-  tree_contains tg tr0 ->
-  tree_contains tgp tr0 ->
-  ~tree_contains tg' tr0 ->
-  reach Reserved (initial_state newp) ->
-  create_child cids0 tgp tg' newp tr0 = Some tr1 ->
-  memory_access AccessWrite ProtStrong cids1 tg range1 tr1 = Some tr2 ->
-  memory_access AccessRead ProtStrong cids2 tg' range2 tr2 = Some tr3 ->
-  ~exists z, range_contains range1 z /\ range_contains range2 z.
-Proof.
-  move=> ? tr0 tr1 tr2 tr3 ??? TgEx TgpEx Tg'Fresh ReachRes Rebor Write12 Read23 [z [RContains1 RContains2]].
-  (* reborrow step *)
-  created tg' unique as [Tg'Ex Tg'Unique].
-  created tg' nonparent of tg as Unrelated.
-  migrate TgEx.
-  forget tr0.
-
-  (* write step 1 *)
-  destruct (nonchild_write_reserved_to_disabled _ _ _ _
-    TgEx Tg'Ex Tg'Unique
-    Unrelated
-    _ _ _ _ _ RContains1 eq_refl
-    ltac:(solve_reachability)
-    Write12
-  ) as [post [zpost [Unique'Post [PermPost [DisPost ProtPost]]]]].
-  migrate Tg'Ex.
-  forget tr1.
-
   (* read step 2 *)
-  destruct (child_read_disabled_to_ub _ _ _ _
-    Tg'Ex Tg'Ex Unique'Post
-    ltac:(left; reflexivity) _ _ _ _ _
+  destruct (child_read_disabled_to_ub
+    Tg'Ex Unique'Post
+    ltac:(left; reflexivity)
     RContains2 PermPost
     ltac:(solve_reachability)
     Read23).
 Qed.
 
 Lemma activated_fread_cwrite_disjoint tg tg' newp range1 range2 range3:
-  forall tgp tr0 tr1 tr2 tr3 tr4 cids0 cids1 cids2 cids3,
+  forall tgp tr0 tr1 tr2 tr3 tr4 cid cids0 cids1 cids2 cids3 cids4,
   tree_contains tg tr0 ->
-  tree_contains tgp tr0 ->
-  ~tree_contains tg' tr0 ->
-  create_child cids0 tgp tg' newp tr0 = Some tr1 ->
-  memory_access AccessWrite ProtStrong cids1 tg' range1 tr1 = Some tr2 ->
-  memory_access AccessRead ProtStrong cids2 tg range2 tr2 = Some tr3 ->
-  memory_access AccessWrite ProtStrong cids3 tg' range3 tr3 = Some tr4 ->
+  bor_local_step tr0 cids0 (RetagBLEvt tgp tg' newp cid) tr1 cids1 ->
+  bor_local_step tr1 cids1 (AccessBLEvt AccessWrite ProtStrong tg' range1) tr2 cids2 ->
+  bor_local_step tr2 cids2 (AccessBLEvt AccessRead ProtStrong tg range2) tr3 cids3 ->
+  bor_local_step tr3 cids3 (AccessBLEvt AccessWrite ProtStrong tg' range3) tr4 cids4 ->
   ~exists z, range_contains range1 z /\ range_contains range2 z /\ range_contains range3 z.
 Proof.
-  move=> ? tr0 tr1 tr2 tr3 tr4 ???? TgEx TgpEx Tg'Fresh Rebor Write12 Read23 Write34 [z [RContains1 [RContains2 RContains3]]].
+  move=> ? tr0 tr1 tr2 tr3 tr4 ?????? TgEx Rebor Write12 Read23 Write34 [z [RContains1 [RContains2 RContains3]]].
   (* reborrow step *)
   created tg' unique as [Tg'Ex Tg'Unique].
   created tg' nonparent of tg as Unrelated.
@@ -536,51 +503,49 @@ Proof.
   forget tr0.
 
   (* write step 1 *)
-  destruct (child_write_any_to_init_active _ _ _ _
-    Tg'Ex Tg'Ex Tg'Unique
+  destruct (child_write_any_to_init_active
+    Tg'Ex Tg'Unique
     ltac:(left; reflexivity)
-    _ _ _ _ RContains1
+    RContains1 eq_refl
     Write12
   ) as [post [zpost [Post'Unique [PostPerm [PostActive _]]]]].
+  migrate Unrelated.
   migrate Tg'Ex.
   migrate TgEx.
-  migrate Unrelated.
   forget tr1.
 
   (* read step 2 *)
   rename post into pre, zpost into zpre.
   rename PostPerm into PrePerm, PostActive into PreActive.
-  destruct (nonchild_read_active_to_frozen _ _ _ _
-    TgEx Tg'Ex Post'Unique
+  destruct (nonchild_read_active_to_frozen
+    Tg'Ex Post'Unique
     Unrelated
-    _ _ _ _ _ RContains2 PrePerm
+    RContains2 PrePerm
     ltac:(solve_reachability)
     Read23) as [post [zpost [Tg'Unique [PostPerm [ReachFrzPost ReachPrePost]]]]].
   migrate Tg'Ex.
   forget tr2.
 
   (* write step 3 *)
-  destruct (child_write_frozen_to_ub _ _ _ _
-    Tg'Ex Tg'Ex Tg'Unique
-    ltac:(left; reflexivity) _ _ _ _ _
+  destruct (child_write_frozen_to_ub
+    Tg'Ex Tg'Unique
+    ltac:(left; reflexivity)
     RContains3 PostPerm
     ltac:(solve_reachability)
     Write34).
 Qed.
 
 Lemma protected_cwrite_fwrite_disjoint tg tg' cid newp range1 range2 :
-  forall tgp tr0 tr1 tr2 tr3 cids0 cids1 cids2,
+  forall tgp tr0 tr1 tr2 tr3 cids0 cids1 cids2 cids3,
   tree_contains tg tr0 ->
-  tree_contains tgp tr0 ->
-  ~tree_contains tg' tr0 ->
   protector_is_for_call (new_protector newp) cid ->
-  create_child cids0 tgp tg' newp tr0 = Some tr1 ->
-  memory_access AccessWrite ProtStrong cids1 tg' range1 tr1 = Some tr2 ->
+  bor_local_step tr0 cids0 (RetagBLEvt tgp tg' newp cid) tr1 cids1 ->
+  bor_local_step tr1 cids1 (AccessBLEvt AccessWrite ProtStrong tg' range1) tr2 cids2 ->
   call_is_active cids2 cid ->
-  memory_access AccessWrite ProtStrong cids2 tg range2 tr2 = Some tr3 ->
+  bor_local_step tr2 cids2 (AccessBLEvt AccessWrite ProtStrong tg range2) tr3 cids3 ->
   ~exists z, range_contains range1 z /\ range_contains range2 z.
 Proof.
-  move=> ? tr0 tr1 tr2 tr3 ?? cids2 TgEx TgpEx Tg'Fresh ProtCall Rebor Write12 CallAct Write23 [z [RContains1 RContains2]].
+  move=> ? tr0 tr1 tr2 tr3 ??? cids2 TgEx ProtCall Rebor Write12 CallAct Write23 [z [RContains1 RContains2]].
   (* reborrow step *)
   created tg' unique as [Tg'Ex Tg'Unique].
   created tg' protected as Protected.
@@ -589,39 +554,38 @@ Proof.
   forget tr0.
 
   (* write step 1 *)
-  destruct (child_write_any_to_init_active _ _ _ _
-    Tg'Ex Tg'Ex Tg'Unique ltac:(left; reflexivity)
-    _ _ _ _ RContains1
+  destruct (child_write_any_to_init_active
+    Tg'Ex Tg'Unique ltac:(left; reflexivity)
+    RContains1 eq_refl
     Write12
   ) as [post [zpost [Post'Unique [PostPerm [PostActive [PostProt PostInit]]]]]].
+  migrate Unrelated.
   migrate TgEx.
   migrate Tg'Ex.
-  migrate Unrelated.
   migrate Protected.
   forget tr1.
 
   subst.
-  destruct (protected_nonchild_write_initialized_to_ub _ _ _ _
-    TgEx Tg'Ex Post'Unique Unrelated
-    _ _ _ _ ltac:(eexists; split; [exact Protected|exact CallAct])
+  destruct (protected_nonchild_write_initialized_to_ub
+    Tg'Ex Post'Unique Unrelated
+    ltac:(eexists; split; [exact Protected|exact CallAct])
     PostInit
-    ltac:(rewrite PostActive; tauto)
-    RContains2 Write23).
+    RContains2 eq_refl
+    ltac:(rewrite PostActive; eauto)
+    Write23).
 Qed.
 
 Lemma protected_cread_fwrite_disjoint tg tg' cid newp range1 range2 :
-  forall tgp tr0 tr1 tr2 tr3 cids0 cids1 cids2,
+  forall tgp tr0 tr1 tr2 tr3 cids0 cids1 cids2 cids3,
   tree_contains tg tr0 ->
-  tree_contains tgp tr0 ->
-  ~tree_contains tg' tr0 ->
   protector_is_for_call (new_protector newp) cid ->
-  create_child cids0 tgp tg' newp tr0 = Some tr1 ->
-  memory_access AccessRead ProtStrong cids1 tg' range1 tr1 = Some tr2 ->
+  bor_local_step tr0 cids0 (RetagBLEvt tgp tg' newp cid) tr1 cids1 ->
+  bor_local_step tr1 cids1 (AccessBLEvt AccessRead ProtStrong tg' range1) tr2 cids2 ->
   call_is_active cids2 cid ->
-  memory_access AccessWrite ProtStrong cids2 tg range2 tr2 = Some tr3 ->
+  bor_local_step tr2 cids2 (AccessBLEvt AccessWrite ProtStrong tg range2) tr3 cids3 ->
   ~exists z, range_contains range1 z /\ range_contains range2 z.
 Proof.
-  move=> ? tr0 tr1 tr2 tr3 ??? TgEx TgpEx Tg'Fresh ProtCall Rebor Read12 CallAct Write23 [z [RContains1 RContains2]].
+  move=> ? tr0 tr1 tr2 tr3 ???? TgEx ProtCall Rebor Read12 CallAct Write23 [z [RContains1 RContains2]].
   (* reborrow step *)
   created tg' unique as [Tg'Ex Tg'Unique].
   created tg' protected as Protected.
@@ -630,36 +594,34 @@ Proof.
   forget tr0.
 
   (* write step 1 *)
-  destruct (child_read_any_to_init_nondis _ _ _ _
-    Tg'Ex Tg'Ex Tg'Unique ltac:(left; reflexivity)
-    _ _ _ _ RContains1 Read12
+  destruct (child_read_any_to_init_nondis
+    Tg'Ex Tg'Unique ltac:(left; reflexivity)
+    RContains1 eq_refl Read12
   ) as [post [zpost [Post'Unique [PostPerm [PostNonDis [PostProt PostInit]]]]]].
+  migrate Unrelated.
   migrate TgEx.
   migrate Tg'Ex.
-  migrate Unrelated.
   migrate Protected.
   forget tr1.
 
   subst.
-  destruct (protected_nonchild_write_initialized_to_ub _ _ _ _
-    TgEx Tg'Ex Post'Unique Unrelated
-    _ _ _ _ ltac:(eexists; split; [exact Protected|exact CallAct])
-    PostInit PostNonDis RContains2 Write23).
+  destruct (protected_nonchild_write_initialized_to_ub
+    Tg'Ex Post'Unique Unrelated
+    ltac:(eexists; split; [exact Protected|exact CallAct])
+    PostInit RContains2 eq_refl PostNonDis Write23).
 Qed.
 
 Lemma protected_cwrite_fread_disjoint tg tg' cid newp range1 range2 :
-  forall tgp tr0 tr1 tr2 tr3 cids0 cids1 cids2,
+  forall tgp tr0 tr1 tr2 tr3 cids0 cids1 cids2 cids3,
   tree_contains tg tr0 ->
-  tree_contains tgp tr0 ->
-  ~tree_contains tg' tr0 ->
   protector_is_for_call (new_protector newp) cid ->
-  create_child cids0 tgp tg' newp tr0 = Some tr1 ->
-  memory_access AccessWrite ProtStrong cids1 tg' range1 tr1 = Some tr2 ->
+  bor_local_step tr0 cids0 (RetagBLEvt tgp tg' newp cid) tr1 cids1 ->
+  bor_local_step tr1 cids1 (AccessBLEvt AccessWrite ProtStrong tg' range1) tr2 cids2 ->
   call_is_active cids2 cid ->
-  memory_access AccessRead ProtStrong cids2 tg range2 tr2 = Some tr3 ->
+  bor_local_step tr2 cids2 (AccessBLEvt AccessRead ProtStrong tg range2) tr3 cids3 ->
   ~exists z, range_contains range1 z /\ range_contains range2 z.
 Proof.
-  move=> ? tr0 tr1 tr2 tr3 ??? TgEx TgpEx Tg'Fresh ProtCall Rebor Write12 CallAct Read23 [z [RContains1 RContains2]].
+  move=> ? tr0 tr1 tr2 tr3 ???? TgEx ProtCall Rebor Write12 CallAct Read23 [z [RContains1 RContains2]].
   (* reborrow step *)
   created tg' unique as [Tg'Ex Tg'Unique].
   created tg' protected as Protected.
@@ -668,35 +630,33 @@ Proof.
   forget tr0.
 
   (* write step 1 *)
-  destruct (child_write_any_to_init_active _ _ _ _
-    Tg'Ex Tg'Ex Tg'Unique ltac:(left; reflexivity)
-    _ _ _ _ RContains1 Write12) as [post [zpost [Post'Unique [PostPerm [PostNonDis [PostProt PostInit]]]]]].
+  destruct (child_write_any_to_init_active
+    Tg'Ex Tg'Unique ltac:(left; reflexivity)
+    RContains1 eq_refl Write12) as [post [zpost [Post'Unique [PostPerm [PostNonDis [PostProt PostInit]]]]]].
+  migrate Unrelated.
   migrate TgEx.
   migrate Tg'Ex.
-  migrate Unrelated.
   migrate Protected.
   forget tr1.
 
   subst.
-  destruct (protected_nonchild_read_initialized_active_to_ub _ _ _ _
-    TgEx Tg'Ex Post'Unique Unrelated
-    _ _ _ _ ltac:(eexists; split; [exact Protected|exact CallAct])
-    PostInit PostNonDis RContains2 Read23).
+  destruct (protected_nonchild_read_initialized_active_to_ub
+    Tg'Ex Post'Unique Unrelated
+    ltac:(eexists; split; [exact Protected|exact CallAct])
+    PostInit RContains2 eq_refl PostNonDis Read23).
 Qed.
 
 Lemma protected_fread_cwrite_disjoint tg tg' cid newp range1 range2 :
-  forall tgp tr0 tr1 tr2 tr3 cids0 cids1 cids2,
+  forall tgp tr0 tr1 tr2 tr3 cids0 cids1 cids2 cids3,
   tree_contains tg tr0 ->
-  tree_contains tgp tr0 ->
-  ~tree_contains tg' tr0 ->
   protector_is_for_call (new_protector newp) cid ->
-  create_child cids0 tgp tg' newp tr0 = Some tr1 ->
+  bor_local_step tr0 cids0 (RetagBLEvt tgp tg' newp cid) tr1 cids1 ->
   call_is_active cids1 cid ->
-  memory_access AccessRead ProtStrong cids1 tg range1 tr1 = Some tr2 ->
-  memory_access AccessWrite ProtStrong cids2 tg' range2 tr2 = Some tr3 ->
+  bor_local_step tr1 cids1 (AccessBLEvt AccessRead ProtStrong tg range1) tr2 cids2 ->
+  bor_local_step tr2 cids2 (AccessBLEvt AccessWrite ProtStrong tg' range2) tr3 cids3 ->
   ~exists z, range_contains range1 z /\ range_contains range2 z.
 Proof.
-  move=> ? tr0 tr1 tr2 tr3 ??? TgEx TgpEx Tg'Fresh ProtCall Rebor CallAct Read12 Write23 [z [RContains1 RContains2]].
+  move=> ? tr0 tr1 tr2 tr3 ???? TgEx ProtCall Rebor CallAct Read12 Write23 [z [RContains1 RContains2]].
   (* reborrow step *)
   created tg' unique as [Tg'Ex Tg'Unique].
   created tg' protected as Protected.
@@ -705,19 +665,19 @@ Proof.
   forget tr0.
 
   (* write step 1 *)
-  destruct (protected_nonchild_read_any_to_frozen _ _ _ _
-    TgEx Tg'Ex Tg'Unique
+  destruct (protected_nonchild_read_any_to_frozen
+    Tg'Ex Tg'Unique
     Unrelated
-    _ _ _ _ ltac:(eexists; split; [exact Protected|exact CallAct])
-    RContains1 Read12
+    ltac:(eexists; split; [exact Protected|exact CallAct])
+    RContains1 eq_refl Read12
   ) as [post [zpost [Unique'Post [PermPost FrzPost]]]].
   migrate Tg'Ex.
   forget tr1.
 
   (* read step 2 *)
-  destruct (child_write_frozen_to_ub _ _ _ _
-    Tg'Ex Tg'Ex Unique'Post
-    ltac:(left; reflexivity) _ _ _ _ _
+  destruct (child_write_frozen_to_ub
+    Tg'Ex Unique'Post
+    ltac:(left; reflexivity)
     RContains2 PermPost
     ltac:(solve_reachability)
     Write23).
